changed the definition of satisfies so that it avoids having everything satisfy spin

coq/handwritten/CryptolToCoq/CompM_ITrees.v
@@ -22,15 +22,18 @@ Definition itree_spec E A : Type := itree (SpecEvent E) A.
 (* The body of an itree_spec, inside the observe projection *)
 Definition itree_spec' E A : Type := itree' (SpecEvent E) A.
 
-Variant satisfiesF {E A} (satisfies : itree_spec E A -> itree E A -> Prop)
+Inductive satisfiesF {E A} (satisfies : itree_spec E A -> itree E A -> Prop)
   : itree_spec' E A -> itree' E A -> Prop :=
 | Satisfies_Ret a : satisfiesF satisfies (RetF a) (RetF a)
+| Satisfies_Tau spec tree :
+    satisfies spec tree ->
+    satisfiesF satisfies (TauF spec) (TauF tree)
 | Satisfies_TauL spec tree :
-    satisfies spec tree ->
-    satisfiesF satisfies (TauF spec) (observe tree)
+    satisfiesF satisfies (observe spec) tree ->
+    satisfiesF satisfies (TauF spec) tree
 | Satisfies_TauR spec tree :
-    satisfies spec tree ->
-    satisfiesF satisfies (observe spec) (TauF tree)
+    satisfiesF satisfies spec (observe tree) ->
+    satisfiesF satisfies spec (TauF tree)
 | Satisfies_Vis X (e:E X) spec tree :
     (forall x, satisfies (spec x) (tree x)) ->
     satisfiesF satisfies (VisF (Spec_vis e) spec) (VisF e tree)
@@ -48,7 +51,8 @@ Instance Proper_satisfies_satisfiesF {E A} :
 Proof.
   intros R1 R2 implR spec1 spec2 e_spec tree1 tree2 e_tree sats.
   rewrite <- e_spec; rewrite <- e_tree.
-  destruct sats; constructor; intros; try (apply implR; apply H).
+  clear e_spec spec2 e_tree tree2.
+  induction sats; constructor; intros; try (apply implR; apply H); try assumption.
   destruct H as [ x H ]. exists x. apply implR; assumption.
 Qed.
 
@@ -67,8 +71,8 @@ Definition satisfies_ {E A} satisfies spec tree :=
 
 Lemma satisfies__mono E A : monotone2 (@satisfies_ E A).
 Proof.
-  intros spec tree r1 r2 sats sub12. unfold satisfies_. destruct sats; constructor.
-  { apply sub12; assumption. }
+  intros spec tree r1 r2 sats sub12. unfold satisfies_.
+  induction sats; constructor; try assumption.
   { apply sub12; assumption. }
   { intros; apply sub12. apply H. }
   { intros; apply sub12. apply H. }
@@ -87,6 +91,11 @@ Proof.
     [ rewrite <- Rtree; rewrite <- Rspec | rewrite Rtree; rewrite Rspec ];
     apply H.
 Qed.
+
+Instance Proper_observing_upaco2_satisfies_impl E A r :
+  Proper (observing eq ==> observing eq ==> iff) (upaco2 (@satisfies_ E A) r).
+Proof.
+Admitted.
 
 Instance Proper_observing_satisfies E A :
   Proper (observing eq ==> observing eq ==> iff) (@satisfies E A).
@@ -107,11 +116,292 @@ Proof.
   intro a. constructor. reflexivity.
 Qed.
 
+(* Two itrees are weakly bisimilar, where we only remove Taus from their heads,
+i.e., before the first non-tau step *)
+Definition eutt_head {E A} (t1 t2:itree E A) : Prop :=
+  eqitF eq true true id eq (observe t1) (observe t2).
+
+(* Two itrees are weakly bisimilar, where we only remove Taus from their tails,
+i.e., after the first non-tau step *)
+Definition eutt_tail {E A} (t1 t2:itree E A) : Prop :=
+  eqitF eq false false id (eutt eq) (observe t1) (observe t2).
+
+(* Split a weak bisimulation into head and tail bits *)
+Lemma eutt_split E A (t1 t2:itree E A) (e:eutt eq t1 t2) :
+  exists2 t1',
+  eutt_head t1 t1' &
+  exists2 t2', eutt_head t2 t2' & eutt_tail t1' t2'.
+Proof.
+  unfold eutt_head, eutt_tail.
+  punfold e. unfold eqit_ in e.
+  revert e. set (obs1 := observe t1). set (obs2 := observe t2).
+  intro e; induction e.
+  { exists (Ret r1); [ reflexivity | ]. exists (Ret r2); [ reflexivity | ].
+    rewrite REL; reflexivity. }
+  { exists (Tau m1); [ reflexivity | ]; exists (Tau m2); [ reflexivity | ].
+    constructor. pclearbot. apply REL. }
+  { exists (Vis e k1); [ reflexivity | ]; exists (Vis e k2); [ reflexivity | ].
+    constructor. intro. pclearbot. apply REL. }
+  { destruct IHe as [ t1' e1 [ t2' e2 e12 ]].
+    exists t1'; [ repeat constructor; assumption | ].
+    exists t2'; [ repeat constructor | ]; assumption. }
+  { destruct IHe as [ t1' e1 [ t2' e2 e12 ]].
+    exists t1'; [ repeat constructor; assumption | ].
+    exists t2'; [ repeat constructor | ]; assumption. }
+Qed.
+
+
+Lemma satisfies_tau_l E A (P:itree_spec E A) m r :
+  paco2 satisfies_ r P m -> paco2 satisfies_ r (Tau P) m.
+Proof.
+  intro sats; pinversion sats.
+  { pfold. constructor. apply sats. }
+  { pfold. constructor. assumption. }
+  { pfold. constructor. rewrite <- H. constructor. assumption. }
+  { rewrite <- (observing_intros _ (Tau tree) _ H). pfold. constructor. left.
+    pfold. assumption. }
+  { rewrite <- (observing_intros _ (Vis _ _) _ H0). pfold. constructor.
+    rewrite <- H. constructor. intro x. apply H1. }
+  { pfold. constructor. rewrite <- H. constructor. intro x.
+    rewrite <- (observing_intros _ _ _ H0). apply H1. }
+  { pfold. constructor. rewrite <- H. constructor.
+    destruct H1 as [ x H1 ]. exists x.
+    rewrite <- (observing_intros _ _ _ H0). assumption. }
+Qed.
+
+
+Lemma satisfies_tau_r E A (P:itree_spec E A) m r :
+  paco2 satisfies_ r P m -> paco2 satisfies_ r P (Tau m).
+Proof.
+  intro sats; pinversion sats.
+  { pfold. constructor. apply sats. }
+  { pfold. constructor. assumption. }
+  { rewrite <- (observing_intros _ (Tau spec) _ H). pfold. constructor. left.
+    pfold. assumption. }
+  { pfold. constructor. rewrite <- H. constructor. assumption. }
+  { rewrite <- (observing_intros _ (Vis _ _) _ H). pfold. constructor.
+    rewrite <- H0. constructor. intro x. apply H1. }
+  { rewrite <- (observing_intros _ (Vis _ _) _ H). pfold. constructor.
+    rewrite <- H0. constructor. intro x. apply H1. }
+  { rewrite <- (observing_intros _ (Vis _ _) _ H). pfold. constructor.
+    rewrite <- H0. destruct H1 as [ x H1 ]. constructor. exists x. assumption. }
+Qed.
+
+Lemma satisfies_inv_tau_l E A (P:itree_spec E A) m r :
+  paco2 satisfies_ r (Tau P) m -> paco2 satisfies_ r P m.
+Proof.
+(*
+  revert P m; pcofix CIH; intros P m sats.
+  punfold sats. revert sats. unfold satisfies_.
+  remember (observe m) as obsm eqn: e_obsm.
+  rewrite <- (observing_intros _ (go obsm) _ e_obsm).
+  remember (observe P) as obsP eqn: e_obsP.
+  simpl. remember (TauF P) as tauP eqn: e_tauP.
+  intro sats. revert P e_tauP e_obsP. induction sats; intros; try discriminate.
+  { injection e_tauP; intro e_P; rewrite e_P in H.
+    pfold. constructor. pclearbot. 
+    
+
+    rewrite e_obsP.
+
+
+  (* remember (observe P2) as obsP2 eqn: e_obsP2 in sats. *)
+  remember (observe tree) as obs_tree eqn: e_obs_tree in sats.
+
+ sats.
+
+pinversion sats.
+  { rewrite <- (observing_intros _ (Tau tree) _ H0).
+    eapply paco2_mon_bot; [ | intros; eassumption ].
+    pfold. constructor. punfold H1. }
+  { eapply paco2_mon_bot; [ | intros; eassumption ].
+    pfold. apply H0. }
+  { pclearbot. 
+
+
+    eapply paco2_mon_bot; [ | intros; eassumption ].
+    pfold. constructor. punfold sats. apply H1.
+
+
+  intro sats; punfold sats. revert sats; unfold satisfies_.
+  remember (observe m) as obsm eqn: e_obsm.
+  remember (observe (Tau P)) as obsTP1 eqn: e_obsTP1.
+  intro sats; revert P m e_obsm e_obsTP1; induction sats; intros; try discriminate.
+  { injection e_obsTP1; intro e_spec. rewrite <- e_spec.
+    rewrite <- (observing_intros _ (Tau tree) _ e_obsm).
+    pfold; pclearbot; punfold H. constructor. apply H. }
+  { injection e_obsTP1; intro e_spec. rewrite <- e_spec.
+
+    injection e_obsm; intro e_m.
+    constructor. pclearbot. apply H.
+
+apply H.
+
+  revert P m; pcofix CIH; intros. punfold H0. unfold satisfies_ in H0.
+  induction 
+*)
+Admitted.
+
+Lemma satisfies_vis_spec_funext E A X e (k1 k2 : X -> itree (SpecEvent E) A) tree r :
+  (forall v, k1 v = k2 v) ->
+  paco2 satisfies_ r (Vis e k1) tree ->
+  paco2 satisfies_ r (Vis e k2) tree.
+Proof.
+  intros funext sats. punfold sats; unfold satisfies_ in sats at 1.
+  simpl in sats. remember (VisF e k1) as obs1 eqn: e_obs1.
+  remember (observe tree) as obs_t eqn: e_obs_t.
+  revert e_obs1 tree e_obs_t. induction sats; intros; try discriminate.
+  { rewrite <- (observing_intros _ (Tau tree) _ e_obs_t). pfold.
+    apply Satisfies_TauR.
+    assert (paco2 satisfies_ r (Vis e k2) tree) as IHapp; [ | punfold IHapp ].
+    apply IHsats; [ assumption | reflexivity ]. }
+  { rewrite <- (observing_intros _ (Vis _ _) _ e_obs_t).
+    destruct e; try discriminate.
+(*
+pfold.
+
+    set (IHapp := IHsats e k1 k2 e_obs1 tree eq_refl). punfold IHapp. }
+  { rewrite <- (observing_intros _ (Vis _ _) _ e_obs_t). pfold.
+    injection e_obs1. intros.
+    dependent rewrite H2.
+    apply Satisfies_Vis.
+
+  clear e_obs_t.
+  intro sats; induction sats; intros; try discriminate.
+*)
+(*
+  { apply satisfies_tau_r.
+    rewrite (observing_intros _ tree0 (go (observe tree0)) eq_refl).
+    apply IHsats; assumption. }
+  { injection e_obs1.
+*)
+Admitted.
+
+Lemma satisfies_eutt_head_spec E A (spec1 spec2:itree_spec E A) tree r :
+  eutt_head spec1 spec2 -> paco2 satisfies_ r spec1 tree -> paco2 satisfies_ r spec2 tree.
+Proof.
+  unfold eutt_head.
+  rewrite (observing_intros _ spec1 (go (observe spec1)) eq_refl).
+  rewrite (observing_intros _ spec2 (go (observe spec2)) eq_refl).
+  set (obs1 := observe spec1). set (obs2 := observe spec2). simpl.
+  intros e sats. induction e.
+  { rewrite <- REL. assumption. }
+  { rewrite <- REL. assumption. }
+  { eapply satisfies_vis_spec_funext; eassumption. }
+  { apply IHe. rewrite (observing_intros _ (go (observe t1)) t1 eq_refl).
+    apply satisfies_inv_tau_l. assumption. }
+  { apply satisfies_tau_l.
+    rewrite (observing_intros _ t2 (go (observe t2)) eq_refl).
+    apply IHe. assumption. }
+Qed.
+
+
+Lemma satisfies_eutt_spec E A (P1 P2:itree_spec E A) tree :
+  satisfies P1 tree -> eutt eq P1 P2 -> satisfies P2 tree.
+Proof.
+  intros 
+
+
+Admitted.
+(*
+  revert P1 P2 tree; pcofix CIH; intros P1 P2 tree sats e12.
+  destruct (eutt_split _ _ _ _ e12) as [ P1' e1 [ P2' e2 e12' ]].
+  eapply satisfies_eutt_head_spec; [ symmetry; eassumption | ].
+  assert (satisfies P1' tree) as sats';
+    [ eapply satisfies_eutt_head_spec; eassumption | ].
+  inversion e12'.
+  { rewrite <- (observing_intros _ (Ret r2) _ H). rewrite <- REL.
+    rewrite (observing_intros _ (Ret r1) _ H0).
+    eapply paco2_mon_bot; [ | intros; eassumption ].
+    assumption. }
+  { rewrite <- (observing_intros _ (Tau _) _ H).
+    rewrite <- (observing_intros _ (Tau _) _ H0) in sats'.
+
+ rewrite <- REL.
+    rewrite (observing_intros _ (Ret r1) _ H0).
+    eapply paco2_mon_bot; [ | intros; eassumption ].
+    assumption. }
+
+
+  punfold sats. unfold satisfies_ in sats.
+  remember (observe P1) as obsP1 eqn: e_obsP1 in sats.
+  (* remember (observe P2) as obsP2 eqn: e_obsP2 in sats. *)
+  remember (observe tree) as obs_tree eqn: e_obs_tree in sats.
+  induction sats. Print eqitF.
+  { eapply paco2_mon_bot; [ | intros; eassumption ].
+    pfold. unfold satisfies_. rewrite <- e_obsP2. rewrite <- REL.
+    punfold sats. unfold satisfies_ in sats.
+    rewrite <- e_obsP1 in sats. apply sats. }
+  { rewrite <- (observing_intros _ (Tau _) _ e_obsP2).
+    pclearbot. pfold.
+*)
+    (*
+    simpl in REL. pfold. unfold satisfies_. rewrite <- e_obsP2. apply Satisfies_TauL.
+
+
+
+
+  revert P1 P2 tree; pcofix CIH; intros P1 P2 tree sats e12.
+  punfold e12. unfold eqit_ in e12.
+  remember (observe P1) as obsP1 eqn: e_obsP1 in e12.
+  remember (observe P2) as obsP2 eqn: e_obsP2 in e12.
+  induction e12.
+  { eapply paco2_mon_bot; [ | intros; eassumption ].
+    pfold. unfold satisfies_. rewrite <- e_obsP2. rewrite <- REL.
+    punfold sats. unfold satisfies_ in sats.
+    rewrite <- e_obsP1 in sats. apply sats. }
+  { rewrite <- (observing_intros _ (Tau _) _ e_obsP2).
+    pclearbot. pfold.
+    (*
+    simpl in REL. pfold. unfold satisfies_. rewrite <- e_obsP2. apply Satisfies_TauL.
+
+    unfold eqit_ in e12. induction e12.
+    *)
+    admit. }
+  { rewrite <- (observing_intros _ (Vis _ _) _ e_obsP2).
+    pclearbot.
+
+
+  { rewrite <- (observing_intros _ (Ret _) _ H). rewrite <- REL.
+    rewrite (observing_intros _ (Ret _) _ H0).
+    eapply paco2_mon_bot; [ apply sats | intros; eassumption ]. }
+  { rewrite <- (observing_intros _ (Tau m2) _ H). pfold. constructor. right.
+    apply (CIH m1).
+    - apply satisfies_inv_tau_l.
+      rewrite (observing_intros _ (Tau m1) _ H0). assumption.
+    - apply REL. }
+  { 
+
+
+
+FIXME HERE: old stuff below
+
+Lemma satisfiesF_exists_eqitF E A r (spec':itree_spec' E A) tree'
+      (sats:satisfiesF r spec' tree') :
+  exists spec, exists tree,
+      eqitF eq true true id eq spec' (observe spec) /\
+      eqitF eq true true id eq tree' (observe tree) /\
+      r spec tree.
+Proof.
+  induction sats.
+  { exists (Ret a); exists (Ret a); split; [ reflexivity | ]; split; [ reflexivity 
+
+
+FIXME HERE: cull the below
 
 Lemma satisfies_inv_tau_l E A (P:itree_spec E A) m :
   satisfies (Tau P) m -> satisfies P m.
 Proof.
-  revert P m; pcofix CIH; intros. punfold H0. inversion H0.
+  revert P m; pcofix CIH; intros. punfold H0.
+
+
+
+  pose (tauP := Tau P). assert (eqP : tauP = Tau P); [ constructor | ].
+  rewrite <- eqP in H0. revert eqP. unfold satisfies_ in H0. induction H0.
+
+induction H0; try rewrite eqP in * |- *; try discriminate.
+  revert H0; pattern (Tau P); intro tauP.
+  induction H0.
   { rewrite <- (observing_intros _ _ _ H1). pclearbot.
     eapply paco2_mon_bot; intros; eassumption. }
   { rewrite <- (observing_intros _ (Tau tree) _ H1). pfold.
@@ -119,10 +409,56 @@ Proof.
     rewrite <- (observing_intros _ _ (Tau P) H). assumption. }
 Qed.
 
-(* FIXME: how do we prove this? *)
-(*
-Instance Proper_eutt_satisfies E A : Proper (eutt eq ==> eutt eq ==> iff) (@satisfies E A).
+
+(* FIXME: no longer needed...? *)
+Lemma observing_spin E A : observing eq (ITree.spin (E:=E) (R:=A)) (Tau ITree.spin).
+Proof.
+  constructor. reflexivity.
+Qed.
+
+
+Lemma satisfies_spin E A (tree:itree E A) : satisfies ITree.spin tree.
+Proof.
+  revert tree; pcofix CIH; intros. pfold.
+  unfold satisfies_. rewrite observing_spin. constructor.
+  right. apply CIH.
+Qed.
+
+Lemma satisfies_inv_ret_l E A a (tree:itree E A) :
+  satisfies (Ret a) tree -> eutt eq tree (Ret a).
+Proof.
+  
+
+  revert tree; pcofix CIH; intros tree sats. pinversion sats.
+  { pfold. unfold eqit_. rewrite <- H. constructor. reflexivity. }
+  { pfold. unfold eqit_. rewrite <- H0. constructor; [ constructor | ]. Print eqitF.
+    
+
+
+rewrite <- (observing_intros _ (Ret a) _ H).
+
+  intro sats. punfold sats. inversion sats. Focus 2.
+
+pinversion sats. Focus 2.
+
+  revert P m; pcofix CIH; intros. punfold H0. inversion H0.
+  { rewrite <- (observing_intros _ _ _ H1). pclearbot.
+    eapply paco2_mon_bot; intros; eassumption. }
+  { rewrite <- (observing_intros _ (Tau tree) _ H1). pfold.
+    apply Satisfies_TauR. right. apply CIH. pclearbot. unfold satisfies.
+    rewrite <- (observing_intros _ _ (Tau P) H). assumption. }
+Qed.
 *)
+
+
+Instance Proper_eutt_satisfies E A : Proper (eutt eq ==> eutt eq ==> iff) (@satisfies E A).
+Proof.
+Admitted.
+
+Instance Proper_eutt_satisfiesF E A r : Proper (eutt eq ==> eutt eq ==> iff)
+                                               (paco2 (@satisfies_ E A) r).
+Proof.
+Admitted.
 
 (* The proposition that a is returned by an itree along some path *)
 Inductive is_itree_retval' {E A} : itree' E A -> A -> Prop :=
@@ -147,6 +483,7 @@ Proof.
   rewrite em. reflexivity.
 Qed.
 
+
 Lemma bind_satisfies_bind E A B (P:itree_spec E A) (Q:A -> itree_spec E B)
       (m:itree E A) (f:A -> itree E B) :
   satisfies P m ->
@@ -154,38 +491,52 @@ Lemma bind_satisfies_bind E A B (P:itree_spec E A) (Q:A -> itree_spec E B)
   satisfies (P >>= Q) (m >>= f).
 Proof.
   intro sats; revert P m sats. pcofix CIH.
-  intros P m sats; punfold sats; inversion sats; intros.
-  { rewrite <- (observing_intros _ (Ret a) _ H).
-    rewrite <- (observing_intros _ (Ret a) _ H0).
+  intros P m sats satsQ; punfold sats. unfold satisfies_ at 1 in sats.
+  remember (observe P) as obsP eqn: e_obsP.
+  remember (observe m) as obsm eqn: e_obsm.
+  revert P m e_obsP e_obsm satsQ. induction sats; intros.
+  { rewrite <- (observing_intros _ (Ret a) _ e_obsP).
+    rewrite <- (observing_intros _ (Ret a) _ e_obsm).
     repeat rewrite bind_ret_.
-    eapply paco2_mon_bot; [ apply H1 | intros; eassumption ].
-    rewrite <- (observing_intros _ (Ret a) _ H). constructor. }
-  { rewrite <- (observing_intros _ (Tau spec) _ H). rewrite bind_tau_.
-    pfold. apply Satisfies_TauL. right. apply CIH; [ | apply H2 ].
-    pclearbot. rewrite <- (observing_intros _ _ _ H0). assumption. }
-  { rewrite <- (observing_intros _ (Tau tree) _ H0). rewrite bind_tau_.
-    pfold. apply Satisfies_TauR. right.
-    apply CIH.
-    - pclearbot. rewrite <- (observing_intros _ _ _ H). assumption.
-    - intros. apply H2. rewrite <- (observing_intros _ (Tau tree) _ H0).
-      constructor. apply H3. }
-  { rewrite <- (observing_intros _ (Vis (Spec_vis e) spec) _ H).
-    rewrite <- (observing_intros _ (Vis e tree) _ H0).
-    rewrite bind_vis_. rewrite bind_vis_. pfold.
-    apply Satisfies_Vis. intro. right. apply CIH.
-    - pclearbot. apply H1.
-    - intros; apply H2. rewrite <- (observing_intros _ (Vis e tree) _ H0).
+    eapply paco2_mon_bot; [ apply satsQ | intros; eassumption ].
+    rewrite <- (observing_intros _ (Ret a) _ e_obsm). constructor. }
+  { rewrite <- (observing_intros _ (Tau _) _ e_obsP).
+    rewrite <- (observing_intros _ (Tau _) _ e_obsm).
+    repeat rewrite bind_tau_.
+    pfold. apply Satisfies_Tau. right. pclearbot. apply CIH; [ assumption | ].
+    intros a iirv. apply satsQ.
+    rewrite <- (observing_intros _ (Tau _) _ e_obsm).
+    constructor. assumption. }
+  { rewrite <- (observing_intros _ (Tau _) _ e_obsP). rewrite bind_tau_.
+    pfold. apply Satisfies_TauL.
+    set (IHapp := IHsats spec m eq_refl e_obsm satsQ). punfold IHapp. }
+  { rewrite <- (observing_intros _ (Tau _) _ e_obsm). rewrite bind_tau_.
+    pfold. apply Satisfies_TauR.
+    assert (paco2 satisfies_ r (P >>= Q) (tree >>= f)) as IHapp;
+      [ | punfold IHapp ].
+    apply IHsats; [ assumption | reflexivity | ].
+    intros. apply satsQ. rewrite <- (observing_intros _ (Tau _) _ e_obsm).
+    constructor. assumption. }
+  { rewrite <- (observing_intros _ (Vis _ _) _ e_obsP).
+    rewrite <- (observing_intros _ (Vis _ _) _ e_obsm).
+    repeat rewrite bind_vis_. pfold.
+    apply Satisfies_Vis. intro x. right. apply CIH.
+    - pclearbot. apply H.
+    - intros. apply satsQ. rewrite <- (observing_intros _ (Vis _ _) _ e_obsm).
       econstructor. eassumption. }
-  { rewrite <- (observing_intros _ (Vis Spec_forall spec) _ H).
+  { rewrite <- (observing_intros _ (Vis _ _) _ e_obsP).
+    rewrite <- (observing_intros _ _ _ e_obsm).
+    rewrite bind_vis_. pfold. apply Satisfies_Forall. intro x. right. apply CIH.
+    - pclearbot. apply H.
+    - intros. apply satsQ.
+      rewrite <- (observing_intros _ _ _ e_obsm). assumption. }
+  { rewrite <- (observing_intros _ (Vis _ _) _ e_obsP).
+    rewrite <- (observing_intros _ _ _ e_obsm).
     rewrite bind_vis_. pfold.
-    apply Satisfies_Forall. intros. right.
-    apply CIH; [ | apply H2 ].
-    pclearbot. rewrite <- (observing_intros _ _ _ H0). apply H1. }
-  { rewrite <- (observing_intros _ (Vis Spec_exists spec) _ H).
-    rewrite bind_vis_. pfold. apply Satisfies_Exists.
-    destruct H1 as [ x sats' ]. exists x. right.
-    apply CIH; [ | apply H2 ].
-    pclearbot. rewrite <- (observing_intros _ _ _ H0). assumption. }
+    destruct H as [ x H ]. apply Satisfies_Exists. exists x. right. apply CIH.
+    - pclearbot. apply H.
+    - intros. apply satsQ.
+      rewrite <- (observing_intros _ _ _ e_obsm). assumption. }
 Qed.
 
 
